---
layout: post
title: A Quick Example of Variational Quantum Eigensolver
tags: physics

---

Take hydrogen molecule $H_2$ as an example, its Hamiltonian $H$ can be written in second quantization as
$$
H=\sum_{i,j}h_{ij}a^\dagger_i a_j+\sum_{i,j,p,q}h_{qpij}a^\dagger_p a^\dagger_qa_ia_j
$$

And with JW-transformation or BK-transformation, (haven't learned this so far)
$$
H=g_0I_0\otimes I_1+g_1Z_0\otimes I_1+g_2I_0\otimes Z_1+g_3Z_0\otimes Z_1+g_4Y_0\otimes Y_1+g_5X_0\otimes X_1,
$$
where, $g_i$'s are determined by the bond length $R$. Now $H$ is expresses as a linear combination of $6$ unitary operators. 



For the experiment, we only need 2 qubits: $q_0$ and $q_1$



1. Prepare the *ansatz* $\vert\psi(\theta)\rangle$

   Let $\vert\psi(\theta)\rangle=a_0\vert00\rangle+a_1\vert01\rangle+a_2\vert10\rangle+a_3\vert11\rangle$. From the experiment, only $P_i=\vert a_i\vert^2$ can be measured after repetitive measurement of polynomial times.

2. Measure the expectation value $\langle\psi(\theta)\vert H\vert\psi(\theta)\rangle$:

   $H=\sum_ig_iH_i$

   $\langle\psi(\theta)\vert H\vert\psi(\theta)\rangle=\sum_ig_i\langle\psi(\theta)\vert H_i\vert\psi(\theta)\rangle$

   - $i=0:\langle\psi(\theta)\vert I_0\otimes I _1\vert\psi(\theta)\rangle=1$

   - $i=1:\langle\psi(\theta)\vert Z_0\otimes I_1\vert\psi(\theta)\rangle=(a_0^*\langle 00\vert+a_1^*\langle 01\vert+a_2^*\langle 10\vert+a_3^*\langle 11\vert)(a_0\vert00\rangle+a_1\vert01\rangle-a_2\vert10\rangle-a_3\vert11\rangle)=P_1+P_2-P_3-P_4$

   - $i=2:\langle\psi(\theta)\vert I_0\otimes Z_1\vert\psi(\theta)\rangle=(a_0^*\langle 00\vert+a_1^*\langle 01\vert+a_2^*\langle 10\vert+a_3^*\langle 11\vert)(a_0\vert00\rangle-a_1\vert01\rangle+a_2\vert10\rangle-a_3\vert11\rangle)=P_1-P_2+P_3-P_4$

   - $i=3:\langle\psi(\theta)\vert Z_0\otimes Z_1\vert\psi(\theta)\rangle=(a_0^*\langle 00\vert+a_1^*\langle 01\vert+a_2^*\langle 10\vert+a_3^*\langle 11\vert)(a_0\vert00\rangle-a_1\vert01\rangle-a_2\vert10\rangle+a_3\vert11\rangle)=P_1-P_2-P_3+P_4$

   - $i=4:\langle\psi(\theta)\vert Y_0\otimes Y_1\vert\psi(\theta)\rangle=(a_0^*\langle 00\vert+a_1^*\langle 01\vert+a_2^*\langle 10\vert+a_3^*\langle 11\vert)(-a_0\vert11\rangle+a_1\vert10\rangle+a_2\vert01\rangle-a_3\vert00\rangle)=\Re[a_1^*a_2-a_0^*a_3]$

     But, this result cannot be measured. So we will need a rotation.

     It can be seen that only with the $Z$ operators can the expection values be obtained.

     Let $\vert\Psi_\phi\rangle=e^{-i\phi X_0\otimes X_1}\vert\psi(\theta)\rangle$. And $\langle\Psi_\phi\vert Z_0\otimes Z_1\vert\Psi_\phi\rangle$is something we can measure.

     $\langle\Psi_\phi\vert Z_0\otimes Z_1\vert\Psi_\phi\rangle=\langle\psi(\theta)\vert e^{i\phi X_0\otimes X_1}Z_0\otimes Z_1e^{-i\phi X_0\otimes X_1} \vert\psi(\theta)\rangle=\langle\psi(\theta)\vert (e^{i\phi X_0}Z_0e^{-i\phi X_0})\otimes (e^{i\phi X_1}Z_1e^{-i\phi X_1})\vert\Psi_\phi\rangle$
     $$
     \begin{eqnarray}
     \nonumber e^{i\phi X_0}Z_0e^{-i\phi X_0}&=&
     \begin{bmatrix}
     \cos\phi & i\sin\phi\\
     i\sin\phi & \cos\phi
     \end{bmatrix}
     \begin{bmatrix}
     1 & 0\\
     0 & -1
     \end{bmatrix}
     \begin{bmatrix}
     \cos\phi & -i\sin\phi\\
     -i\sin\phi & \cos\phi
     \end{bmatrix}\\
     \nonumber &=&
     \begin{bmatrix}
     \cos2\phi & -i\sin2\phi\\
     i\sin2\phi & -\cos2\phi
     \end{bmatrix}\\
     \nonumber &=&\cos2\phi Z_0+\sin2\phi Y_0
     \end{eqnarray}
     $$
     So by choosing $\phi=\frac{\pi}{4},e^{i\pi X_0/4}Z_0e^{-i\pi X_0/4}=Y_0$, we get
     $$
     \langle\psi(\theta)\vert Y_0\otimes Y_1\vert\psi(\theta)\rangle=\langle\psi(\theta)\vert e^{i\pi X_0\otimes X_1/4}Z_0\otimes Z_1e^{-i\pi X_0\otimes X_1/4}\vert\psi(\theta)\rangle=\langle\Psi_{\pi/4}\vert Z_0\otimes Z_1\vert\Psi_{\pi/4}\rangle
     $$
     All we need to do now is to apply a $R_x(\pi/2)$ to the ansatz and then use $P_1'-P_2'-P_3'+P_4'$ as the expection value, with $P_i'$ being the probabilty distribution for $\vert\Psi_{\pi/4}\rangle$.

   - $i=5$, use $R_y(\pi/2)$ instead.

   This step need 5 different circuits, but they share a same input state $\vert\psi(\theta)\rangle$.

3. Minimize the target function $f(\theta)=\langle\psi(\theta)\vert H\vert\psi(\theta)\rangle$ by using algorithms like gradient descent.



Finally we can obtain both $\vert\psi(\theta_0)\rangle$and its corresponding energy $E_0$.